\begin{problema}
    \kant[1]
\end{problema}
\solution

\kant[1-3]

\begin{align*}
    m^{2}\ddot{x}\dot{x}^{2} + 2m\ddot{x}V(x) + 2m\dot{x}^{2}V^{\prime}(x) - m\dot{x}^{2}V^{\prime}(x) + 2V(x)V^{\prime}(x) &= 0,\\
    m^{2}\ddot{x}\dot{x}^{2} + 2m\ddot{x}V(x) + m\dot{x}^{2}V^{\prime}(x) + 2V(x)V^{\prime}(x) &= 0,\\
    \dfrac{1}{2}\left[(m\dot{x}^{2} + 2V(x))m\ddot{x} + (m\dot{x}^{2} + 2V(x))V^{\prime}(x)\right] &= 0,\\
    \left(\dfrac{1}{2}m\dot{x}^{2} + V(x)\right)m\ddot{x} + \left(\dfrac{1}{2}m\dot{x}^{2} + V(x)\right)V^{\prime}(x) &= 0,\\
    \textcolor{blue}{\left(\dfrac{1}{2}m\dot{x}^{2} + V(x)\right)}\textcolor{red}{(m\ddot{x} + V^{\prime}(x))} &= 0.
\end{align*}